code/ecdsap256/Hacl.Spec.P256.MontgomeryMultiplication.fst
@@ -4,131 +4,130 @@ open FStar.Mul
 
 module S = Spec.P256
 
-#set-options "--z3rlimit 40 --fuel 0 --ifuel 0"
+#set-options "--z3rlimit 50 --fuel 0 --ifuel 0"
 
-let mont_R = pow2 256
-let mont_R_inv = S.modp_inv2_prime (pow2 256) S.prime
+let fmont_R = pow2 256
+let fmont_R_inv = S.modp_inv2_prime (pow2 256) S.prime
 
-let fromDomain_ (a:int) : S.felem = a * mont_R_inv % S.prime
-let toDomain_   (a:int) : S.felem = a * mont_R % S.prime
+let from_mont (a:int) : S.felem = a * fmont_R_inv % S.prime
+let to_mont   (a:int) : S.felem = a * fmont_R % S.prime
 
-let fromDomainPoint (a:tuple3 nat nat nat) : S.jacob_point =
-  let x, y, z = a in
-  fromDomain_ x, fromDomain_ y, fromDomain_ z
+let from_mont_point (a:tuple3 nat nat nat) : S.jacob_point =
+  let x, y, z = a in from_mont x, from_mont y, from_mont z
 
 
-val lemmaToDomainAndBackIsTheSame: a:S.felem -> Lemma (fromDomain_ (toDomain_ a) == a)
+val lemmaToDomainAndBackIsTheSame: a:S.felem -> Lemma (from_mont (to_mont a) == a)
 let lemmaToDomainAndBackIsTheSame a =
   calc (==) {
-    fromDomain_ (toDomain_ a); // == a
+    from_mont (to_mont a); // == a
     (==) { }
-    (a * mont_R % S.prime) * mont_R_inv % S.prime;
-    (==) { Math.Lemmas.lemma_mod_mul_distr_l (a * mont_R) mont_R_inv S.prime }
-    a * mont_R * mont_R_inv % S.prime;
-    (==) { Math.Lemmas.paren_mul_right a mont_R mont_R_inv }
-    a * (mont_R * mont_R_inv) % S.prime;
-    (==) { Math.Lemmas.lemma_mod_mul_distr_r a (mont_R * mont_R_inv) S.prime }
-    a * (mont_R * mont_R_inv % S.prime) % S.prime;
-    (==) { assert_norm (mont_R * mont_R_inv % S.prime = 1) }
+    (a * fmont_R % S.prime) * fmont_R_inv % S.prime;
+    (==) { Math.Lemmas.lemma_mod_mul_distr_l (a * fmont_R) fmont_R_inv S.prime }
+    a * fmont_R * fmont_R_inv % S.prime;
+    (==) { Math.Lemmas.paren_mul_right a fmont_R fmont_R_inv }
+    a * (fmont_R * fmont_R_inv) % S.prime;
+    (==) { Math.Lemmas.lemma_mod_mul_distr_r a (fmont_R * fmont_R_inv) S.prime }
+    a * (fmont_R * fmont_R_inv % S.prime) % S.prime;
+    (==) { assert_norm (fmont_R * fmont_R_inv % S.prime = 1) }
     a % S.prime;
     (==) { Math.Lemmas.modulo_lemma a S.prime }
     a;
   }
 
 
-val lemmaFromDomainToDomain: a:S.felem -> Lemma (toDomain_ (fromDomain_ a) == a)
+val lemmaFromDomainToDomain: a:S.felem -> Lemma (to_mont (from_mont a) == a)
 let lemmaFromDomainToDomain a =
   calc (==) {
-    toDomain_ (fromDomain_ a); // == a
+    to_mont (from_mont a); // == a
     (==) { }
-    (a * mont_R_inv % S.prime) * mont_R % S.prime;
-    (==) { Math.Lemmas.lemma_mod_mul_distr_l (a * mont_R_inv) mont_R S.prime }
-    a * mont_R_inv * mont_R % S.prime;
-    (==) { Math.Lemmas.paren_mul_right a mont_R_inv mont_R }
-    a * (mont_R_inv * mont_R) % S.prime;
-    (==) { Math.Lemmas.lemma_mod_mul_distr_r a (mont_R_inv * mont_R) S.prime }
-    a * (mont_R_inv * mont_R % S.prime) % S.prime;
-    (==) { assert_norm (mont_R_inv * mont_R % S.prime = 1) }
+    (a * fmont_R_inv % S.prime) * fmont_R % S.prime;
+    (==) { Math.Lemmas.lemma_mod_mul_distr_l (a * fmont_R_inv) fmont_R S.prime }
+    a * fmont_R_inv * fmont_R % S.prime;
+    (==) { Math.Lemmas.paren_mul_right a fmont_R_inv fmont_R }
+    a * (fmont_R_inv * fmont_R) % S.prime;
+    (==) { Math.Lemmas.lemma_mod_mul_distr_r a (fmont_R_inv * fmont_R) S.prime }
+    a * (fmont_R_inv * fmont_R % S.prime) % S.prime;
+    (==) { assert_norm (fmont_R_inv * fmont_R % S.prime = 1) }
     a % S.prime;
     (==) { Math.Lemmas.modulo_lemma a S.prime }
     a;
   }
 
 
-val inDomain_mod_is_not_mod: a:int -> Lemma (toDomain_ a == toDomain_ (a % S.prime))
+val inDomain_mod_is_not_mod: a:int -> Lemma (to_mont a == to_mont (a % S.prime))
 let inDomain_mod_is_not_mod a =
   calc (==) {
-    toDomain_ (a % S.prime); // == toDomain_ a
+    to_mont (a % S.prime);
     (==) { }
-    (a % S.prime) * mont_R % S.prime;
-    (==) { Math.Lemmas.lemma_mod_mul_distr_l a mont_R S.prime }
-    a * mont_R % S.prime;
+    (a % S.prime) * fmont_R % S.prime;
+    (==) { Math.Lemmas.lemma_mod_mul_distr_l a fmont_R S.prime }
+    a * fmont_R % S.prime;
   }
 
 
 val fmont_mul_lemma: a:S.felem -> b:S.felem ->
-  Lemma (S.fmul (fromDomain_ a) (fromDomain_ b) = fromDomain_ ((a * b * mont_R_inv) % S.prime))
+  Lemma (S.fmul (from_mont a) (from_mont b) = from_mont ((a * b * fmont_R_inv) % S.prime))
 
 let fmont_mul_lemma a b =
   calc (==) {
-    (fromDomain_ a * fromDomain_ b) % S.prime;
+    (from_mont a * from_mont b) % S.prime;
     (==) { }
-    ((a * mont_R_inv % S.prime) * (b * mont_R_inv % S.prime)) % S.prime;
+    ((a * fmont_R_inv % S.prime) * (b * fmont_R_inv % S.prime)) % S.prime;
     (==) { Math.Lemmas.lemma_mod_mul_distr_l
-      (a * mont_R_inv) (b * mont_R_inv % S.prime) S.prime }
-    (a * mont_R_inv * (b * mont_R_inv % S.prime)) % S.prime;
-    (==) { Math.Lemmas.lemma_mod_mul_distr_r (a * mont_R_inv) (b * mont_R_inv) S.prime }
-    (a * mont_R_inv * (b * mont_R_inv)) % S.prime;
-    (==) { Math.Lemmas.paren_mul_right a mont_R_inv (b * mont_R_inv) }
-    (a * (mont_R_inv * (b * mont_R_inv))) % S.prime;
-    (==) { Math.Lemmas.paren_mul_right mont_R_inv b mont_R_inv }
-    (a * (mont_R_inv * b * mont_R_inv)) % S.prime;
-    (==) { Math.Lemmas.swap_mul mont_R_inv b }
-    (a * (b * mont_R_inv * mont_R_inv)) % S.prime;
-    (==) { Math.Lemmas.paren_mul_right a (b * mont_R_inv) mont_R_inv }
-    (a * (b * mont_R_inv) * mont_R_inv) % S.prime;
-    (==) { Math.Lemmas.paren_mul_right a b mont_R_inv }
-    (a * b * mont_R_inv * mont_R_inv) % S.prime;
-    (==) { Math.Lemmas.lemma_mod_mul_distr_l (a * b * mont_R_inv) mont_R_inv S.prime }
-    fromDomain_ ((a * b * mont_R_inv) % S.prime);
+      (a * fmont_R_inv) (b * fmont_R_inv % S.prime) S.prime }
+    (a * fmont_R_inv * (b * fmont_R_inv % S.prime)) % S.prime;
+    (==) { Math.Lemmas.lemma_mod_mul_distr_r (a * fmont_R_inv) (b * fmont_R_inv) S.prime }
+    (a * fmont_R_inv * (b * fmont_R_inv)) % S.prime;
+    (==) { Math.Lemmas.paren_mul_right a fmont_R_inv (b * fmont_R_inv) }
+    (a * (fmont_R_inv * (b * fmont_R_inv))) % S.prime;
+    (==) { Math.Lemmas.paren_mul_right fmont_R_inv b fmont_R_inv }
+    (a * (fmont_R_inv * b * fmont_R_inv)) % S.prime;
+    (==) { Math.Lemmas.swap_mul fmont_R_inv b }
+    (a * (b * fmont_R_inv * fmont_R_inv)) % S.prime;
+    (==) { Math.Lemmas.paren_mul_right a (b * fmont_R_inv) fmont_R_inv }
+    (a * (b * fmont_R_inv) * fmont_R_inv) % S.prime;
+    (==) { Math.Lemmas.paren_mul_right a b fmont_R_inv }
+    (a * b * fmont_R_inv * fmont_R_inv) % S.prime;
+    (==) { Math.Lemmas.lemma_mod_mul_distr_l (a * b * fmont_R_inv) fmont_R_inv S.prime }
+    from_mont ((a * b * fmont_R_inv) % S.prime);
   }
 
 
 val fmont_add_lemma: a:S.felem -> b:S.felem ->
-  Lemma (S.fadd (fromDomain_ a) (fromDomain_ b) = fromDomain_ ((a + b) % S.prime))
+  Lemma (S.fadd (from_mont a) (from_mont b) = from_mont ((a + b) % S.prime))
 
 let fmont_add_lemma a b =
   calc (==) {
-    (fromDomain_ a + fromDomain_ b) % S.prime;
+    (from_mont a + from_mont b) % S.prime;
     (==) { }
-    (a * mont_R_inv % S.prime + b * mont_R_inv % S.prime) % S.prime;
-    (==) { Math.Lemmas.modulo_distributivity (a * mont_R_inv) (b * mont_R_inv) S.prime }
-    (a * mont_R_inv + b * mont_R_inv) % S.prime;
-    (==) { Math.Lemmas.distributivity_add_left a b mont_R_inv }
-    (a + b) * mont_R_inv % S.prime;
-    (==) { Math.Lemmas.lemma_mod_mul_distr_l (a + b) mont_R_inv S.prime }
-    (a + b) % S.prime * mont_R_inv % S.prime;
+    (a * fmont_R_inv % S.prime + b * fmont_R_inv % S.prime) % S.prime;
+    (==) { Math.Lemmas.modulo_distributivity (a * fmont_R_inv) (b * fmont_R_inv) S.prime }
+    (a * fmont_R_inv + b * fmont_R_inv) % S.prime;
+    (==) { Math.Lemmas.distributivity_add_left a b fmont_R_inv }
+    (a + b) * fmont_R_inv % S.prime;
+    (==) { Math.Lemmas.lemma_mod_mul_distr_l (a + b) fmont_R_inv S.prime }
+    (a + b) % S.prime * fmont_R_inv % S.prime;
     (==) { }
-    fromDomain_ ((a + b) % S.prime);
+    from_mont ((a + b) % S.prime);
   }
 
 
 val fmont_sub_lemma: a:S.felem -> b:S.felem ->
-  Lemma (S.fsub (fromDomain_ a) (fromDomain_ b) = fromDomain_ ((a - b) % S.prime))
+  Lemma (S.fsub (from_mont a) (from_mont b) = from_mont ((a - b) % S.prime))
 
 let fmont_sub_lemma a b =
   calc (==) {
-    (fromDomain_ a - fromDomain_ b) % S.prime;
+    (from_mont a - from_mont b) % S.prime;
     (==) { }
-    (a * mont_R_inv % S.prime - b * mont_R_inv % S.prime) % S.prime;
-    (==) { Math.Lemmas.lemma_mod_sub_distr (a * mont_R_inv % S.prime) (b * mont_R_inv) S.prime }
-    (a * mont_R_inv % S.prime - b * mont_R_inv) % S.prime;
-    (==) { Math.Lemmas.lemma_mod_plus_distr_l (a * mont_R_inv) (- b * mont_R_inv) S.prime }
-    (a * mont_R_inv - b * mont_R_inv) % S.prime;
-    (==) { Math.Lemmas.distributivity_sub_left a b mont_R_inv }
-    (a - b) * mont_R_inv % S.prime;
-    (==) { Math.Lemmas.lemma_mod_mul_distr_l (a - b) mont_R_inv S.prime }
-    (a - b) % S.prime * mont_R_inv % S.prime;
+    (a * fmont_R_inv % S.prime - b * fmont_R_inv % S.prime) % S.prime;
+    (==) { Math.Lemmas.lemma_mod_sub_distr (a * fmont_R_inv % S.prime) (b * fmont_R_inv) S.prime }
+    (a * fmont_R_inv % S.prime - b * fmont_R_inv) % S.prime;
+    (==) { Math.Lemmas.lemma_mod_plus_distr_l (a * fmont_R_inv) (- b * fmont_R_inv) S.prime }
+    (a * fmont_R_inv - b * fmont_R_inv) % S.prime;
+    (==) { Math.Lemmas.distributivity_sub_left a b fmont_R_inv }
+    (a - b) * fmont_R_inv % S.prime;
+    (==) { Math.Lemmas.lemma_mod_mul_distr_l (a - b) fmont_R_inv S.prime }
+    (a - b) % S.prime * fmont_R_inv % S.prime;
     (==) { }
-    fromDomain_ ((a - b) % S.prime);
+    from_mont ((a - b) % S.prime);
   }
